---
layout: single
title: "[Fourier 1] The Genesis of Fourier Analysis"
categories: mathematics
tags: [analysis, Fourier analysis, Fourier Series]
use_math: true
publish: false
author_profile: false
toc: true
---

# Chapter 1. The Genesis of Fourier Series

## 1. The vibrating string

## 2. The Heat Equation

## 3. Exercises

### 3.1
The absolute value of $z=x+iy$ where $x,y\in\mathbb R$ is

$$|z| = \sqrt{x^2+y^2}.$$

(a) Geometrically, we can think of $z$ as a point $(x,y)$ in the plane $\mathbb R^2$.
In this sense, $|z|$ is the distance between two points $(0,0)$ and $(x,y)$.

(b) If $|z|=0$, then $z=0$.

Suppose that $\sqrt{x^2+y^2}=0$.
It follows that $x^2+y^2=0$ and $x=y=0$.
Thus $z=0$.

(c) If $\lambda\in\mathbb R$, then $|\lambda z|=|\lambda||z|$.

$$|\lambda z|=|\lambda x + i(\lambda y)|
=\sqrt{\lambda^2x^2+\lambda^2y^2}
=|\lambda|\sqrt{x^2+y^2}
=|\lambda||z|.$$

(d) $|z_1z_2|=|z_1||z_2|,\quad|z_1+z_2|\le|z_1|+|z_2|$

Since
$$
\begin{align*}
|z_1z_2|^2
&=\left|(x_1+iy_1)(x_2+iy_2)\right|^2\\
&=\left|(x_1x_2-y_1y_2)+i(x_1y_2+x_2y_1)\right|^2\\
&=(x_1x_2-y_1y_2)^2+(x_1y_2+x_2y_1)^2\\
&={x_1}^2{x_2}^2+{y_1}^2{y_2}^2+{x_1}^2{y_2}^2+{y_1}^2{x_2}^2\\
&=\left({x_1}^2+{y_1}^2\right)\left({x_2}^2+{y_2}^2\right)\\
&=|z_1|^2|z_2|^2,
\end{align*}
$$
It follows that $|z_1z_2|=|z_1||z_2|$.

The second statement is equivalent to the following inequalities ;

$$
\begin{align*}
\left(|z_1|+|z_2|\right)^2&\ge|z_1+z_2|^2\\
\left(\sqrt{{x_1}^2+{y_1}^2}+\sqrt{{x_2}^2+{y_2}^2}\right)^2&\ge(x_1+x_2)^2+(y_1+y_2)^2\\
2\sqrt{{x_1}^2+{y_1}^2}\sqrt{{x_2}^2+{y_2}^2}&\ge2x_1x_2+2y_1y_2\\
\left({x_1}^2+{y_1}^2\right)\left({x_2}^2+{y_2}^2\right)&\ge\left(x_1x_2+y_1y_2\right)^2\\
\left(x_1y_2-x_2y_1\right)^2&\ge0\\
\end{align*}
$$
Since the last inequality holds for every $z_1$ and $z_2$, the original statement also holds for every $z_1$ and $z_2$.

(e) If $z\ne0$, then $|1/z|=1/|z|$

$$
\begin{align*}
\left|\frac 1z\right|
&=\left|\frac 1{x+iy}\right|\\
&=\left|\frac {x-iy}{x^2+y^2}\right|\\
&=\frac1{x^2+y^2}|x-iy|\\
&=\frac1{x^2+y^2}\sqrt{x^2+y^2}\\
&=\frac1{\sqrt{x^2+y^2}}\\
&=\frac1{|z|}
\end{align*}
$$

### 3.2
The complex conjugate of $z=x+iy$ is

$$\bar z = x-iy.$$

(a) Geometrically, $\bar z$ is the reflected point $(x,-y)$ of the original point $(x,y)$ through the x-axis.

(b) $|z|^2=z\bar z$

$$z\bar z = (x+iy)(x-iy)=x^2-(iy)^2=x^2+y^2=|z|^2$$

(c) If $z$ belongs to the unit circle, then $1/z=\bar z$.

Since $|z|=1$, we have $z\bar z=|z|^2=1$, where we can divide $z$ on both side.

### 3.3
(a)
A complex sequence $\{w_n\}_{n=1}^\infty$ converges to $w$ or $w_n\to w$ if

$$\lim_{n\to\infty}|w_n-w|=0.$$

Show that the limit is unique.

Suppose that $w_n\to w$ and $w_n\to w'$ where $w\ne w'$.
Since $\frac{|w-w'|}3>0$, there exists $N$ and $N'$ such that
$$
\begin{align*}
n>N&\quad\Longrightarrow\quad|w_n-w|<\frac{|w-w'|}3\\
n>N'&\quad\Longrightarrow\quad|w_n-w'|<\frac{|w-w'|}3\\
\end{align*}
$$
Now if $n>\max(N,N')$, then

$$
\begin{align*}
|w-w'|
&=\left|w_n-w\right|+\left|w_n-w'\right|\\
&<\frac{|w-w'|}3 + \frac{|w-w'|}3\\
&=\frac{2|w-w'|}3
\end{align*}
$$

It follows that $|w-w'|<0$.
This contradiction implies that the limit is unique.

(b) Prove that $\{w_n\}$ is Cauchy iff it is convergent.

Suppose that $\{w_n\}$ is convergent, say, to $w$.
Fix $\epsilon>0$.
Take $N$ so that 

$$n>N\quad\Longrightarrow\quad |w_n-w|<\frac\epsilon2.$$

If $m>n>N$, then

$$|w_m-w_n|\le|w_m-w|+|w_n-w|<\frac\epsilon2+\frac\epsilon2=\epsilon.$$
It follows that $\{w_n\}$ is Cauchy.

Suppose on the contrary that $\{w_n\}$ is Cauchy.
Writing $w_n=x_n+iy_n$, it is immediate that $\{x_n\}$ and $\{y_n\}$ are also Cauchy.
Since $\mathbb R$ is complete, $\{x_n\}$ and $\{y_n\}$ are convergent, say, to $x$ and $y$, respectively.
Fix $\epsilon>0$.
There exist $N$ such that if $n>N$, then

$$
\begin{align*}
|x_n-x|&<\frac{\epsilon}2\\
|y_n-y|&<\frac{\epsilon}2\\
\end{align*}
$$

It follows that 

$$
\begin{align*}
|w_n-w|
&=\left|(x_n-x)+i(y_n-y)\right|\\
&\le|x_n-x|+|i(y_n-y)|\\
&=|x_n-x|+|y_n-y|\\
&<\epsilon.
\end{align*}
$$

Thus, $w_n\to w$.

(c) [Comparison Test] A series $\sum_{n=1}^\infty z_n$ converges if the partial sums

$$S_N = \sum_{n=1}^Nz_n$$

converges.

Prove that if $\{a_n\}$ is a nonnegative sequence whose series $\sum a_n$ converges such that $|z_n|\le a_n$ for all $n$, then $\sum z_n$ also converges.

<!-- It is enough to prove that for any $\epsilon>0$, there exists $N>0$ such that if $m>n>N$, then

$$\left|S_m-S_n\right|<\epsilon.$$

Note that $S_m-S_n=\sum_{i=n+1}^mz_n$. -->

Since $\sum a_n$ converges, the partial sum of $\{a_n\}$ converges and it is Cauchy.
Thus, there exists $N>0$ such that if $m>n>N$, then

$$\sum_{i=n+1}^ma_n <\epsilon.$$

Then, if $m>n>N$,

$$|S_m-S_n|=\left|\sum_{i=n+1}^mz_n\right| \le \sum_{i=n+1}^m|z_n| \le \sum_{i=n+1}^ma_n <\epsilon.$$

Therefore, the $\{S_n\}$ is Cauchy and is convergent.
It follows that $\sum z_n$ is convergent.

### 3.4
Define the exponential function as a power series as follows ;

$$e^z=\sum_{n=0}^\infty\frac{z^n}{n!}$$

(a) Prove that the above sum is always convergent.
Moreover show that the convergence is uniform on every bounded subset $S$ of $\mathbb C$.

Fix $z\in C$ and apply the ratio test;
$$
\lim_{n\to\infty}\frac{\frac{z^{n+1}}{(n+1)!}}{\frac{z^n}{n!}}
=\lim_{n\to\infty}\frac{z}{n+1}=0.
$$
Thus, the power series is convergent.

Now, exclude the case when $S=\varnothing$.
Let $M=\sup\{|s|:s\in S\}$ so that $0\le M<\infty$.
Denote
$$f_n(z)=\sum_{k=1}^n\frac{z^k}{k!}.$$
We know that $f_n\to f$ pointwisely where $f(z)=e^z$, and we are to prove that $f_n\to f$ uniformly.

Fix $\epsilon>0$.
Note that the summation
$$\sum_{n=0}^\infty\frac{M^n}{n!}$$
converges by another ratio test.
That is, there exists $N$ such that if $m>n>N$, then

$$\sum_{k=n+1}^m\frac{M^k}{k!}<\epsilon.$$

Now, if $z\in S$ and $m>n>N$, then

$$
\begin{align*}
\left|f_m(z)-f_n(z)\right|
&=\left|\sum_{k=n+1}^m\frac{z^k}{k!}\right|\\
&\le\sum_{k=n+1}^m\frac{|z|^k}{k!}\\
&\le\sum_{k=n+1}^m\frac{M^k}{k!}\\
&<\epsilon.
\end{align*}
$$

That is, $\{f_n\}$ is Cauchy and thus convergent.

With the $N$ corresponding to the $\epsilon>0$, if $n>N$ and $z\in S$, then

$$
\begin{align*}
\left|f(z)-f_n(z)\right|
&=\left|\lim_{m\to\infty}f_m(z)-f_n(z)\right|\\
&=\lim_{m\to\infty}\left|f_m(z)-f_n(z)\right|\\
&\le\epsilon
\end{align*}
$$

Therefore, $f_n\to f$ uniformly.

(전체적인 증명은 [Weierstrauss M-test](https://en.wikipedia.org/wiki/Weierstrass_M-test)를 참고하였음.)

(b) Prove that $e^{z_1+z_2}=e^{z_1}e^{z_2}$

[Confer baby rudin 3.48, 3.50]

$$
\begin{align*}
e^{z_1}e^{z_2}
&=\sum_{n=0}^\infty\frac{{z_1}^n}{n!}\sum_{n=0}^\infty\frac{{z_2}^n}{n!}\\
&=\sum_{n=0}^\infty\sum_{k=0}^n\frac{{z_1}^k}{k!}\frac{{z_2}^{n-k}}{(n-k)!}\\
&=\sum_{n=0}^\infty\frac1{n!}\sum_{k=0}^n\binom nk{z_1}^k{z_2}^{n-k}\\
&=\sum_{n=0}^\infty\frac1{n!}(z_1+z_2)^n\\
&=e^{z_1+z_2}
\end{align*}
$$

(c) Derive Euler's identity.

Taylor's theorem aplied to sine and cosine yields

$$
\begin{align*}
\cos t = 1-\frac{t^2}{2!}+\frac{t^4}{4!}-\frac{t^6}{6!}+\cdots\\
\cos t = 1-\frac{t^2}{2!}+\frac{t^4}{4!}-\frac{t^6}{6!}+\cdots\\

\end{align*}
$$

Plug in $x=0$ in the equation in (a) to get

$$e^{}$$